\subsection{Transformation of the Horizontal Momentum Equations } \label{der:hor-mom2-sig}

According to difference rule
\begin{align}
\spbt\dudt &= \fd{(\spbt u)}{t} - u\fd{\spbt}{t} \notag\\
&= \fd{U}{t} - u\fd{\spbt}{t} \label{eq:26}
\end{align}

From the mass conservation equation (\ref{eq:8}), we have
\begin{align}
\fd{\pbt}{t} + \pbt\divv &= 0 \notag\\
2\spbt\fd{\spbt}{t} + \pbt\divv &= 0 \notag\\
\fd{\spbt}{t} &= -\f{\spbt}{2}\divv \label{eq:25}
\end{align}

Substitute (\ref{eq:25}) into (\ref{eq:26}), get
\begin{align}
\spbt\dudt &= \pUpt + \vv\cdot\gn U + \f{U}{2}\divv \notag\\
&= \pUpt + \gn\cdot(U\vv) - \f{U}{2}\divv \notag\\
&= \pUpt + \mm(U)
\end{align}
where the advection operator $\mm$ is defined as
\beeq \label{eq:29}
\mm(U) = \gn\cdot(U\vv) - \f{U}{2}\divv
\eneq

Similar to (\ref{eq:11}), we express the divergence operator in pressure-$\gs$
coordinate, get
\begin{align}
\mm(U) &= \racosf\fp{(uU)}{\gl} + \racosf\fp{(vU\cosf)}{\gf} + \fp{(\dgs U)}{\gs}
\notag\\
&- \f{U}{2}\grpp{ \racosf \pupl + \racosf \fp{(v\cosf)}{\gf} + \fp{\dgs}{\gs} }
\notag\\
&= \racosf \grpp{ \fp{(uU)}{\gl} - \f{U}{2}\pupl + \fp{(vU\cosf)}{\gf} -
\f{U}{2} \fp{(v\cosf)}{\gf} } \notag\\
&+\grpp{ \fp{(\dgs U)}{\gs} - \f{U}{2}\fp{\dgs}{\gs} }
\end{align}
