\subsection{Vertical Velocity Equation}
\label{der:sig-w}

Integrate the mass conservation equation (\ref{eq:8}) from the surface to an
arbitary vertical depth
\beeq
\intzs \grpp{ \pppt+\racosf\ppupl+\racosf\ppvcpf+\ppsps }d\gs=0
\eneq
\beeq 
\pppt \gs + \racosf \intzs \grpp{ \ppupl + \ppvcpf }d\gs + 
\pbt \dgs - (\pbt\dgs)_{\gs=0} = 0
\eneq
So
\beeq \label{eq:35}
\pbt\dgs = (\pbt\dgs)_{\gs=0} - \gs\pppt - \racosf\intzs\grpp{ \ppupl + \ppvcpf }d\gs
\eneq

From (\ref{eq:28}), we get
\beeq \label{eq:36}
\pppt = -\rz g \fep - \racosf \grpp{ \fp{(P U_b)}{\gl} + \fp{(P V_b\cosf)}{\gf}
}.
\eneq
Substitute (\ref{eq:36}) into (\ref{eq:35}), we have
\begin{align}
  \pbt\dgs &= -\rz g \fep + \gs\rz g\fep + \racosf\intzs d\gs
  \grpp{ \fp{(\spbt U_b)}{\gl} + \fp{(\spbt V_b\cosf)}{\gf} } \notag\\
  &-\racosf\intzs \grpp{ \fp{(\spbt U)}{\gl} + \fp{(\spbt V\cosf)}{\gf} }\notag\\
  &=\racosf\intzs\grppp{ \fp{[\spbt (U_b-U)]}{\gl} + \fp{[\spbt
  (V_b-V)\cosf]}{\gf} } -(1-\gs)\rz g\fep
\end{align}
